theory/Game/NoWorse.v
@@ -1,0 +1,151 @@
+Require Import Games.Game.Game.
+Require Import Games.Game.Player.
+Require Import Games.Game.Strategy.
+Require Import Games.Game.Win.
+Require Import Games.Game.Draw.
+
+CoInductive no_worse {G : Game} (p : Player) : GameState G -> Type :=
+  | atom_draw_no_worse : forall s,
+      atomic_res s = Some Draw ->
+      no_worse p s
+  | atom_win_no_worse : forall s,
+      atomic_res s = Some (Win p) ->
+      no_worse p s
+  | eloise_no_worse : forall s,
+      atomic_res s = None ->
+      to_play s = p ->
+      forall m, no_worse p (exec_move s m) ->
+      no_worse p s
+  | abelard_no_worse : forall s,
+      atomic_res s = None ->
+      to_play s = opp p ->
+      (forall m, no_worse p (exec_move s m)) ->
+      no_worse p s.
+
+CoInductive weak_draw {G : Game} : GameState G -> Type :=
+  | atom_weak_draw : forall s,
+      atomic_res s = Some Draw ->
+      weak_draw s
+  | eloise_weak_draw : forall s p,
+      atomic_res s = None ->
+      to_play s = p ->
+      (forall m, no_worse (opp p) (exec_move s m)) ->
+      forall m, weak_draw (exec_move s m) ->
+      weak_draw s.
+
+CoFixpoint weak_draw_no_worse {G : Game} (p : Player) : forall (s : GameState G),
+  weak_draw s -> no_worse p s.
+Proof.
+  intros s wd_s.
+  destruct wd_s.
+  - apply atom_draw_no_worse; auto.
+  - destruct (player_id_or_opp_r_t p0 p).
+    + rewrite e1 in *.
+      eapply eloise_no_worse; auto.
+      apply weak_draw_no_worse; eauto.
+    + rewrite e1 in *.
+      apply abelard_no_worse; auto.
+      rewrite opp_invol in n.
+      exact n.
+Defined.
+
+CoFixpoint both_no_worse_weak_draw {G : Game} : forall p (s : GameState G),
+  no_worse p s -> no_worse (opp p) s -> weak_draw s.
+Proof.
+  intros p s nw_ps nw_ops.
+  destruct (atomic_res s) eqn:s_res.
+  - destruct r.
+    + destruct (player_id_or_opp_r_t p0 p).
+      * rewrite e in *.
+        destruct nw_ops; try congruence.
+        elim (opp_no_fp p); congruence.
+      * rewrite e in *.
+        destruct nw_ps; try congruence.
+        elim (opp_no_fp p); congruence.
+    + apply atom_weak_draw; auto.
+  - destruct nw_ps; try congruence.
+    + destruct nw_ops; try congruence.
+      * elim (opp_no_fp p); congruence.
+      * eapply eloise_weak_draw; eauto.
+        rewrite opp_invol; auto.
+    + destruct nw_ops; try congruence.
+      * eapply eloise_weak_draw; eauto.
+        rewrite opp_invol; auto.
+      * elim (opp_no_fp (opp p)); congruence.
+Defined.
+
+Record NW_Trap {G} (P : GameState G -> Type) p := {
+  NWT_no_loss : forall s, P s -> atomic_res s <> Some (Win (opp p));
+  NWT_eloise : forall s, P s -> atomic_res s = None -> to_play s = p ->
+    { m : Move s & P (exec_move s m) };
+  NWT_abelard : forall s, P s -> atomic_res s = None -> to_play s = opp p ->
+    forall m, P (exec_move s m)
+  }.
+
+CoFixpoint NW_Trap_nw {G} {P : GameState G -> Type} {p} : NW_Trap P p ->
+  forall s, P s -> no_worse p s.
+Proof.
+  intros PT s p_s.
+  destruct (atomic_res s) eqn:s_res.
+  - destruct r.
+    + apply atom_win_no_worse.
+      rewrite s_res; repeat f_equal.
+      destruct (player_id_or_opp_r_t p0 p); auto.
+      rewrite e in s_res.
+      elim (NWT_no_loss _ _ PT s); auto.
+    + apply atom_draw_no_worse; auto.
+  - destruct (player_id_or_opp_r_t (to_play s) p).
+    + destruct (NWT_eloise _ _ PT s) as [m Hm]; auto.
+      eapply eloise_no_worse; auto.
+      eapply NW_Trap_nw; eauto.
+    + apply abelard_no_worse; auto.
+      intro m.
+      eapply NW_Trap_nw; eauto.
+      eapply NWT_abelard; eauto.
+Defined.
+
+Lemma no_worse_not_lost {G : Game} (p : Player) : forall (s : GameState G), no_worse p s ->
+  win (opp p) s -> False.
+Proof.
+  intros s nw_s w_s.
+  induction w_s.
+  - destruct nw_s; try congruence.
+    elim (opp_no_fp p); congruence.
+  - apply IHw_s.
+    destruct nw_s; try congruence.
+    + elim (opp_no_fp p); congruence.
+    + apply n.
+  - destruct nw_s; try congruence.
+    + apply (H m); exact nw_s.
+    + elim (opp_no_fp (opp p)); congruence.
+Qed.
+
+Lemma win_no_worse {G : Game} (p : Player) : forall (s : GameState G), win p s ->
+ no_worse p s.
+Proof.
+  intros s w_s.
+  induction w_s.
+  - apply atom_win_no_worse; auto.
+  - eapply eloise_no_worse; eauto.
+  - apply abelard_no_worse; auto.
+Qed.
+
+CoFixpoint draw_no_worse {G : Game} (p : Player) : forall (s : GameState G), draw s ->
+  no_worse p s.
+Proof.
+  intros s s_draw.
+  destruct s_draw.
+  - apply atom_draw_no_worse; auto.
+  - destruct (player_id_or_opp_r_t p0 p).
+    + rewrite e1 in *.
+      eapply eloise_no_worse; auto.
+      apply draw_no_worse. exact s_draw.
+    + rewrite e1 in *.
+      apply abelard_no_worse; auto.
+      intro m'.
+      destruct (s0 m').
+      * apply draw_no_worse. exact d.
+      * apply win_no_worse.
+        rewrite opp_invol in w.
+        exact w.
+Defined.
