theory/Game/Result.v
@@ -1,0 +1,230 @@
+Require Import Games.Game.Game.
+Require Import Games.Game.Player.
+Require Import Games.Game.Strategy.
+
+CoInductive Res :=
+  | Win_res (pl : Player) : Res
+  | Step_res : Res -> Res.
+
+Definition Res_id (r : Res) : Res :=
+  match r with
+  | Win_res pl => Win_res pl
+  | Step_res r' => Step_res r'
+  end.
+
+Lemma Res_id_eq (r : Res) : r = Res_id r.
+Proof.
+  destruct r; reflexivity.
+Qed.
+
+CoInductive bisim : Res -> Res -> Prop :=
+  | Win_refl {pl} : bisim (Win_res pl) (Win_res pl)
+  | Step_bisim {r1 r2} : bisim r1 r2 -> bisim (Step_res r1) (Step_res r2).
+
+CoFixpoint draw : Res := Step_res draw.
+
+Definition Res_of_Result (r : Result) : Res :=
+  match r with
+  | Win pl => Win_res pl
+  | Draw => draw
+  end.
+
+Fixpoint Res_of_n pl (n : nat) : Res :=
+  match n with
+  | 0 => Win_res pl
+  | S m => Step_res (Res_of_n pl m)
+  end.
+
+Definition Res_of_tb_res (o : option (Player * nat)) : Res :=
+  match o with
+  | Some (pl, n) => Res_of_n pl n
+  | None => draw
+  end.
+
+CoInductive res_le (pl : Player) : Res -> Res -> Prop :=
+  | Win_is_best : forall r, res_le pl r (Win_res pl)
+  | Loss_is_worst : forall r, res_le pl (Win_res (opp pl)) r
+  | Step_mon : forall r1 r2, res_le pl r1 r2 -> res_le pl (Step_res r1) (Step_res r2).
+
+Notation "r1 <<= p r2" := (res_le p r1 r2)
+  (at level 10, r2 at next level, p at next level).
+
+CoFixpoint res_flip pl : forall r1 r2,
+  r1 <<= pl r2 -> r2 <<= (opp pl) r1.
+Proof.
+  intros r1 r2 H.
+  destruct H.
+  - rewrite <- (opp_invol pl) at 2.
+    apply Loss_is_worst.
+  - apply Win_is_best.
+  - apply Step_mon.
+    now apply res_flip.
+Defined.
+
+Axiom cheat : forall {X}, X.
+
+CoFixpoint res_le_trans_pf pl : forall r1 r2 r3,
+  r1 <<= pl r2 -> r2 <<= pl r3 -> r1 <<= pl r3.
+Proof.
+  intros r1 r2 r3 H1 H2.
+  destruct H1.
+  - apply cheat.
+
+  - apply Loss_is_worst.
+  - destruct r3.
+    + apply cheat.
+    + apply Step_mon.
+      eapply (res_le_trans_pf).
+      * exact H1.
+      * apply cheat.
+Defined.
+
+Print res_le_trans_pf.
+
+Definition res_le_trans pl :=
+
+let cofix res_le_trans_pf
+  (r1 r2 r3 : Res) (H1 : r1 <<= pl r2) (H2 : r2 <<= pl r3) :
+    r1 <<= pl r3 :=
+  match H1 in (r <<= _ r0) return (r0 <<= pl r3 -> r <<= pl r3) with
+  | Win_is_best _ r => (fun (r0 : Res) (_ : (Win_res pl) <<= pl r3) => cheat) r
+  | Loss_is_worst _ r =>
+      (fun (r0 : Res) (_ : r0 <<= pl r3) => Loss_is_worst pl r3) r
+  | Step_mon _ r4 r5 x =>
+      (fun (r6 r7 : Res) (H3 : r6 <<= pl r7) (H4 : (Step_res r7) <<= pl r3) =>
+       match
+         r3 as r return ((Step_res r7) <<= pl r -> (Step_res r6) <<= pl r)
+       with
+       | Win_res pl0 =>
+           (fun (pl1 : Player) (_ : (Step_res r7) <<= pl (Win_res pl1)) => cheat)
+             pl0
+       | Step_res r =>
+           (fun (r8 : Res) (_ : (Step_res r7) <<= pl (Step_res r8)) =>
+            Step_mon pl r6 r8 (res_le_trans_pf r6 r7 r8 H3 cheat)) r
+       end H4) r4 r5 x
+  end H2 in
+  res_le_trans_pf.
+
+
+(*
+CoFixpoint res_le_trans pl : forall r1 r2 r3,
+  r1 <<= pl r2 -> r2 <<= pl r3 -> r1 <<= pl r3.
+Proof.
+  intros r1 r2 r3 H1 H2.
+  destruct H2 eqn:?.
+  - apply Win_is_best.
+  - inversion H1.
+    + elim (opp_no_fp pl); congruence.
+    + apply Loss_is_worst.
+  - destruct r1.
+    + inversion H1.
+      apply Loss_is_worst.
+    + apply Step_mon.
+      apply (res_le_trans pl _ r0); auto.
+      now inversion H1.
+Defined.
+
+
+Axiom cheat : forall {X},X.
+
+Goal res_le_trans = cheat.
+*)
+
+CoFixpoint res_le_antisym pl : forall r1 r2,
+  r1 <<= pl r2 -> r2 <<= pl r1 ->
+  bisim r1 r2.
+Proof.
+  intros.
+  destruct H.
+  - inversion H0.
+    + apply Win_refl.
+    + elim (opp_no_fp pl); congruence.
+  - inversion H0.
+    + elim (opp_no_fp pl); congruence.
+    + apply Win_refl.
+  - inversion H0.
+    apply Step_bisim.
+    apply (res_le_antisym _ _ _ H H3).
+Qed.
+
+Lemma atomic_res_inf {G} (s : GameState G) :
+  { r : Result & atomic_res s = Some r } +
+  (atomic_res s = None) .
+Proof.
+  destruct atomic_res as [r|].
+  - left; exists r; reflexivity.
+  - right; reflexivity.
+Defined.
+
+CoFixpoint trace {G} {pl} {s : GameState G}
+  (s1 : strategy pl s) (s2 : strategy (opp pl) s) : Res.
+Proof.
+  destruct (atomic_res_inf s) as [[r s_res]|s_res].
+  - exact (Res_of_Result r).
+  - apply Step_res.
+    destruct s1; try congruence.
+    + destruct s2; try congruence; try (elim (opp_no_fp pl); congruence).
+      exact (trace _ _ _ s1 (s m)).
+    + destruct s2; try congruence; try (elim (opp_no_fp (opp pl)); congruence).
+      exact (trace _ _ _ (s m) s2).
+Defined.
+
+CoFixpoint opp_opp_str {G} {pl} {s : GameState G} (st : strategy pl s) : strategy (opp (opp pl)) s.
+Proof.
+  destruct st.
+  - eapply atom_strategy; eauto.
+  - eapply eloise_strategy; auto.
+    + now rewrite opp_invol.
+    + apply opp_opp_str.
+      exact st.
+  - apply abelard_strategy; auto.
+    now rewrite opp_invol.
+Defined.
+
+CoFixpoint bisim_refl : forall r, bisim r r.
+Proof.
+  intro r.
+  destruct r; constructor.
+  apply bisim_refl.
+Defined.
+
+CoFixpoint trace_comm {G} {pl} {s : GameState G}
+  (s1 : strategy pl s) (s2 : strategy (opp pl) s) :
+  bisim (trace s1 s2) (trace s2 (opp_opp_str s1)).
+Proof.
+  rewrite (Res_id_eq (trace s1 s2)).
+  rewrite (Res_id_eq (trace s2 (opp_opp_str s1))).
+  unfold Res_id.
+  unfold trace.
+  destruct (atomic_res_inf s) as [[r s_res]|s_res].
+  - apply bisim_refl.
+  - constructor.
+    destruct s1; try (elim (opp_no_fp pl); congruence).
+    + destruct s2; try (elim (opp_no_fp (opp pl)); congruence).
+      fold @trace.
+      unfold opp_opp_str.
+      fold @opp_opp_str.
+      apply trace_comm.
+    + destruct s2; try (elim (opp_no_fp (opp pl)); congruence).
+      fold @trace.
+      unfold opp_opp_str.
+      fold @opp_opp_str.
+      apply trace_comm.
+Defined.
+
+Definition str_le {G} {st : GameState G} {pl} (s s' : strategy pl st) : Prop :=
+  forall opp, exists opp', (trace s opp') <<= pl (trace s' opp).
+
+Notation "s <<= s'" := (str_le s s')
+  (at level 10).
+
+Definition optimal {G} {pl} {s : GameState G} (str : strategy pl s) : Prop :=
+  forall str', str' <<= str.
+
+
+
+
+
+
+
+
